src/QueryStructure/Implementation/DataStructures/BagADT/BagADT.v
@@ -17,9 +17,10 @@ Section BagADT.
   Variable MatchSearchTerm : SearchTermType -> ElementType -> bool.
   Variable ApplyUpdateTerm : UpdateTermType -> ElementType -> ElementType.
 
+  (* Get rid of Bag. *)
   Definition BagSig : ADTSig :=
     ADTsignature {
-        Constructor "EmptyBag" : unit             -> rep,
+        Constructor "Empty" : unit             -> rep,
         Method "Find"      : rep x SearchTermType -> rep x list ElementType,
         Method "Enumerate" : rep x unit -> rep x list ElementType,
         Method "Insert"    : rep x ElementType -> rep x unit,
@@ -28,25 +29,27 @@ Section BagADT.
         Method "Update"    : rep x (SearchTermType * UpdateTermType) -> rep x unit
   }.
 
+  (* Indentation? *)
+
   Definition BagSpec : ADT BagSig :=
     ADTRep (IndexedEnsemble) {
-        Def Constructor "EmptyBag" (_ : unit) : rep :=
+        Def Constructor "Empty" (_ : unit) : rep :=
           ret (Empty_set _),
 
         Def Method "Find" (r : rep, f : SearchTermType)
           : list ElementType :=
             results <- {l | EnsembleIndexedListEquivalence r l};
-        ret (r, filter (MatchSearchTerm f) results),
+            ret (r, filter (MatchSearchTerm f) results),
 
         Def Method "Enumerate" (r : rep, f : unit)
           : list ElementType :=
             results <- {l | EnsembleIndexedListEquivalence r l};
-        ret (r, results),
+            ret (r, results),
 
         Def Method "Insert" (r : rep, element : ElementType) : unit :=
           freshIdx <- {freshIdx | UnConstrFreshIdx r freshIdx};
-        ret (Add _ r {| elementIndex := freshIdx;
-                        indexedElement := element |}, ()),
+          ret (Add _ r {| elementIndex := freshIdx;
+                          indexedElement := element |}, ()),
 
         Def Method "Count" (r : rep, f : SearchTermType) : nat :=
           results <- {l | EnsembleIndexedListEquivalence r l};
